data/isabelle/src/ESPLogic/InferenceRules.thy
@@ -76,6 +76,7 @@ where
       (nextRel (filter (\<lambda> x. \<not> (noteStep x)) (takeWhile (\<lambda> x. x \<noteq> step) R) @ [step]) st st') \<longrightarrow>
       ((recvStep st \<longrightarrow> (\<exists> m. Some m = inst s i (stepPat st) \<and> predOrd t (Ln m) (St (i, st)))) \<and>
        (matchEqStep st \<longrightarrow> Some (s (matchVar st, i)) = inst s i (stepPat st)) \<and>
+       (notMatchStep st \<longrightarrow> Some (s (matchVar st, i)) \<noteq> inst s i (stepPat st)) \<and>
        predOrd t (St (i, st)) (St (i, st')))
    )"
 
@@ -237,6 +238,10 @@ lemma prefixClose_rawI:
     \<lbrakk> nextRel (filter (\<lambda> x. \<not> (noteStep x)) (takeWhile (\<lambda> x. x \<noteq> step) R) @ [step]) st st';
       matchEqStep st
     \<rbrakk> \<Longrightarrow> Some (s (matchVar st, i)) = inst s i (stepPat st)"
+  and "\<And> st st'.
+    \<lbrakk> nextRel (filter (\<lambda> x. \<not> (noteStep x)) (takeWhile (\<lambda> x. x \<noteq> step) R) @ [step]) st st';
+      notMatchStep st
+    \<rbrakk> \<Longrightarrow> Some (s (matchVar st, i)) \<noteq> inst s i (stepPat st)"
   and "\<And> st st'. 
     \<lbrakk> nextRel (filter (\<lambda> x. \<not> (noteStep x)) (takeWhile (\<lambda> x. x \<noteq> step) R) @ [step]) st st'
     \<rbrakk> \<Longrightarrow> St (i, st) \<prec> St (i, st')"
@@ -302,6 +307,12 @@ proof -
         using steps by (auto dest!: matchEqStepD Match_eq)
     }
     note match_eq = this
+    {
+      assume "notMatchStep st"
+      hence "Some (s (matchVar st, i)) \<noteq> inst s i (stepPat st)"
+        using steps by (auto dest!: notMatchStepD Not_Match)
+    }
+    note not_match = this
 
     have "listOrd R st st'" 
       using nextRel and R_split and done_split
@@ -311,7 +322,7 @@ proof -
       apply -
       apply(drule this_thread.in_steps_conv_done_skipped[THEN iffD1])
       by(fastforce dest!: this_thread.roleOrd_notSkipped_imp_listOrd_trace dest:listOrd_imp_predOrd)+
-    note input and match_eq and this
+    note input and match_eq and not_match and this
   }
   ultimately show ?thesis
     by (auto simp: prefixClose_def)
@@ -323,13 +334,15 @@ lemma ext_prefixClose:
   "\<lbrakk> (i, step) \<in> steps t; roleMap r i = Some R \<rbrakk> \<Longrightarrow>
    prefixClose s t R step i \<and> 
    (recvStep step \<longrightarrow> (\<exists> m. Some m = inst s i (stepPat step) \<and> Ln m \<prec> St (i, step))) \<and>
-   (matchEqStep step \<longrightarrow> Some (s (matchVar step, i)) = inst s i (stepPat step))"
-by (cases step) (auto dest: prefixCloseI Ln_before_inp matchEqStepD Match_eq)
+   (matchEqStep step \<longrightarrow> Some (s (matchVar step, i)) = inst s i (stepPat step)) \<and>
+   (notMatchStep step \<longrightarrow> Some (s (matchVar step, i)) \<noteq> inst s i (stepPat step))"
+by (cases step) (auto dest: prefixCloseI Ln_before_inp matchEqStepD Match_eq notMatchStepD Not_Match)
 
 text{* 
   Used for prefix closing assumptions corresponding to a case of
   an annotation completeness induction proof.
 *}
+(* TODO clean up and merge *)
 lemma thread_prefixClose:
   assumes thread_exists: "r i = Some (step#done, todo, skipped)"
       and not_skipped:   "step \<notin> skipped"
@@ -339,14 +352,21 @@ lemma thread_prefixClose:
           (\<exists> m. Some m = inst s i (stepPat st) \<and> predOrd t (Ln m) (St (i, st)))
         ) \<and>
        (matchEqStep st \<longrightarrow> Some (s (matchVar st, i)) = inst s i (stepPat st)) \<and>
-        predOrd t (St (i, st)) (St (i, st')))
+       (notMatchStep st \<longrightarrow> Some (s (matchVar st, i)) \<noteq> inst s i (stepPat st)) \<and>
+       predOrd t (St (i, st)) (St (i, st')))
     ) \<and>
     (recvStep (last (step#done)) \<longrightarrow>
        (\<exists> m. Some m = inst s i (stepPat (last (step#done))) \<and>
              predOrd t (Ln m) (St (i, (last (step#done))))
        )
+    ) \<and>
+    (matchEqStep (last (step#done)) \<longrightarrow>
+        Some (s (matchVar (last (step#done)), i)) = inst s i (stepPat (last (step#done)))
+    ) \<and>
+    (notMatchStep (last (step#done)) \<longrightarrow>
+        Some (s (matchVar (last (step#done)), i)) \<noteq> inst s i (stepPat (last (step#done)))
     )"
-  (is "?prefix \<and> ?inp_last")
+  (is "?prefix \<and> ?inp_last \<and> ?match_eq_last \<and> ?not_match_last")
 proof -
   interpret this_thread: reachable_thread P t r s i "step#done" todo skipped
     using thread_exists by unfold_locales auto
@@ -362,8 +382,37 @@ proof -
           using thread_exists recv_eq
           by(fastforce dest!: this_thread.in_steps_recv[THEN iffD1])
         qed
-    hence "?inp_last"
-      by (cases "last (step # done)") (fastforce dest!: Ln_before_inp)+
+    hence "?inp_last" by (fastforce dest: recvStepD Ln_before_inp)
+  }
+  moreover
+  {
+    assume match: "matchEqStep (last (step#done))"
+    hence last_step: "(i, last (step#done)) \<in> steps t"
+      proof -
+        obtain l v pt
+          where match_eq: "(Match l True v pt) = (last (step # done))"
+          using match by (fastforce dest!: matchEqStepD)
+        hence "Match l True v pt \<in> set (step # done)" by auto
+        thus ?thesis
+          using thread_exists match_eq
+          by(fastforce dest!: this_thread.in_steps_recv[THEN iffD1])
+        qed
+     hence "?match_eq_last" by (fastforce dest: matchEqStepD Match_eq)
+  }
+  moreover
+  {
+    assume match: "notMatchStep (last (step#done))"
+    hence last_step: "(i, last (step#done)) \<in> steps t"
+      proof -
+        obtain l v pt
+          where match_eq: "(Match l False v pt) = (last (step # done))"
+          using match by (fastforce dest!: notMatchStepD)
+        hence "Match l False v pt \<in> set (step # done)" by auto
+        thus ?thesis
+          using thread_exists match_eq
+          by(fastforce dest!: this_thread.in_steps_recv[THEN iffD1])
+        qed
+     hence "?not_match_last" by (fastforce dest: notMatchStepD Not_Match)
   }
   moreover
   { 
@@ -420,11 +469,15 @@ proof -
     from step_ord have matchEq:
         "matchEqStep st \<Longrightarrow> Some (s (matchVar st, i)) = inst s i (stepPat st)"
       using this_thread.roleMap
-      by (cases st) (auto dest: Ln_before_inp in_steps_predOrd1 matchEqStepD Match_eq)
-    note step_ord recv matchEq
+      by (cases st) (auto dest: in_steps_predOrd1 matchEqStepD Match_eq)
+    from step_ord have notMatch:
+        "notMatchStep st \<Longrightarrow> Some (s (matchVar st, i)) \<noteq> inst s i (stepPat st)"
+      using this_thread.roleMap
+      by (cases st) (auto dest: in_steps_predOrd1 notMatchStepD Not_Match)
+    note step_ord recv matchEq notMatch
   }
   ultimately
-  show ?thesis by fast
+  show ?thesis by blast
 qed
 
 end
